src/FS/MailServerLayers.v
@@ -3,11 +3,289 @@ Require Import FSModel.
 Require Import LinkAPI.
 Require Import FSAPI.
 Require Import MailServerAPI.
+Require Import FMapInterface.
+Require Import FMapAVL.
+Require Import OrderedTypeEx.
 
 Import ListNotations.
 Require Import String.
 Open Scope string.
 Open Scope list.
+
+
+(* Abstraction: directories are limited to [tmp] or [mail; user] *)
+
+Module LinkDirAPI <: Layer.
+
+  Inductive user :=
+  | User0
+  | User1.
+
+  Inductive mfs_dir :=
+  | MFStmp : mfs_dir
+  | MFSuser : forall (u : user), mfs_dir.
+
+
+  Instance mfs_dir_equal : EqualDec mfs_dir.
+  Admitted.
+
+(*
+  Module mfs_dir_as_OT <: UsualOrderedType.
+    Definition t := mfs_dir.
+
+    Definition eq := @eq t.
+    Definition eq_refl := @eq_refl t.
+    Definition eq_sym := @eq_sym t.
+    Definition eq_trans := @eq_trans t.
+
+    Definition lt (x y : t) : Prop.
+    Admitted.
+
+    Theorem lt_trans : forall x y z : t, lt x y -> lt y z -> lt x z.
+    Admitted.
+
+    Theorem lt_not_eq : forall x y, lt x y -> ~ eq x y.
+    Admitted.
+
+    Definition compare x y : OrderedType.Compare lt eq x y.
+    Proof.
+    Admitted.
+
+    Definition eq_dec : forall (x y : t), {x=y}+{x<>y}.
+    Admitted.
+
+  End mfs_dir_as_OT.
+
+  Module Dirs := FMapAVL.Make(mfs_dir_as_OT).
+*)
+
+  Module DirContents := FMapAVL.Make(String_as_OT).
+
+  Definition mfs_dir_contents := DirContents.t nat.
+
+  Record mfs_state := mkMFS {
+    MFSLinks : mfs_dir -> mfs_dir_contents;
+    MFSFiles : Files;
+  }.
+
+  Definition State := mfs_state.
+
+  Inductive mfs_opT : Type -> Type :=
+  | FindAvailable (pfx : string) (d : mfs_dir) : mfs_opT (option string)
+  | CreateFile (d : mfs_dir) (fn : string) : mfs_opT (option nat)
+  | FileRead (f : nat) : mfs_opT (option string)
+  | FileWrite (f : nat) (data : string) : mfs_opT (option unit)
+  | LinkToUser (srcfn : string) (dstfn : string) (user : string) : mfs_opT (option unit)
+  | UnlinkTmp (fn : string) : mfs_opT (option unit)
+  | ListUser (user : string) : mfs_opT (option (list string))
+  | LookupUser (user : string) (fn : string) : mfs_opT (option nat).
+
+  Definition opT := mfs_opT.
+
+  Definition initP (s : State) := True.
+
+  Definition file_handle_unused (fs : State) h :=
+    ~ exists d name, DirContents.find name ((MFSLinks fs) d) = Some h.
+
+  Definition file_handle_valid (fs : State) h :=
+    h < Datatypes.length (MFSFiles fs).
+
+  Definition add_link dir fid name (fs : State) :=
+    mkMFS
+      (fun d' =>
+        if d' == dir then
+          DirContents.add name fid (MFSLinks fs dir)
+        else
+          MFSLinks fs d')
+      (MFSFiles fs).
+
+  Inductive xstep : forall T, opT T -> nat -> State -> T -> State -> Prop :=
+(*
+  | StepFindAvailable : forall pfx d state res tid,
+    DirContents.find res ((MFSLinks state) d) = None ->
+    xstep (FindAvailable pfx d) tid
+      state
+      (Some res)
+      state
+*)
+  | StepCreateFile : forall d fn state fid tid,
+    DirContents.find fn ((MFSLinks state) d) = None ->
+    file_handle_valid state fid ->
+    file_handle_unused state fid ->
+    xstep (CreateFile d fn) tid
+      state
+      (Some fid)
+      (add_link d fid fn state)
+  .
+
+  Definition step := xstep.
+
+End LinkDirAPI.
+
+
+Module LinkDirStableAPI <: Layer.
+
+  Definition opT := LinkAPI.opT.
+  Definition State := LinkAPI.State.
+  Definition initP := LinkAPI.initP.
+
+  Inductive op_allow : forall T, linkOpT T -> nat -> LinkAPI.State -> Prop :=
+  | OpAllowLinkAllocFile : forall dirnum name tid fs_state,
+    op_allow (LinkAllocFile dirnum name) tid fs_state
+
+  | OpAllowLinkLookup : forall dirnum name tid fs_state,
+    op_allow (LinkLookup dirnum name) tid fs_state
+
+  | OpAllowFileWrite : forall tid fs_state f data,
+    op_allow (FileWrite f data) tid fs_state
+
+  | OpAllowFileRead : forall tid fs_state f,
+    op_allow (FileRead f) tid fs_state
+
+  | OpAllowLinkTmp : forall dirnum dirname name f tid fs_state,
+    path_eval_root fs_state [dirname] (DirNode dirnum) ->
+    op_allow (LinkAdd dirnum name (FileNode f)) tid fs_state
+
+  | OpAllowUnlink : forall dirnum dirname name f tid fs_state,
+    path_eval_root fs_state [dirname] (DirNode dirnum) ->
+    valid_link fs_state dirnum name (FileNode f) ->
+    op_allow (LinkDel dirnum name (FileNode f)) tid fs_state
+
+  | OpAllowReaddir : forall dirnum tid fs_state,
+    op_allow (LinkList dirnum) tid fs_state
+
+(*
+  | MailAllowFindUser : forall dirnum tid fs_state user pfx,
+    starts_with_tid tid pfx ->
+    path_eval_root fs_state [maildir; user] (DirNode dirnum) ->
+    mailfs_step_allowed (LinkFindUnusedName dirnum pfx) tid fs_state
+
+  | MailAllowFindTmp : forall dirnum tid fs_state pfx,
+    starts_with_tid tid pfx ->
+    path_eval_root fs_state [tmpdir] (DirNode dirnum) ->
+    mailfs_step_allowed (LinkFindUnusedName dirnum pfx) tid fs_state
+*)
+
+  | OpAllowGetTID : forall state tid,
+    op_allow GetTID tid state
+
+  | OpAllowLinkGetRoot : forall state tid,
+    op_allow LinkGetRoot tid state
+  .
+
+  Definition step := nilpotent_step LinkAPI.step op_allow.
+
+  Definition loopInv (s : State) (tid : nat) := True.
+
+End LinkDirStableAPI.
+
+
+Module Dirs <: LayerImpl LinkDirAPI LinkAPI.
+
+  Import LinkDirAPI.
+
+  Definition user_to_dirname (u : user) :=
+    match u with
+    | User1 => "user1"
+    | User2 => "user2"
+    end.
+
+  Definition dir_to_pn (d : mfs_dir) :=
+    [ match d with
+      | MFStmp => "tmp"
+      | MFSuser u => user_to_dirname u
+      end ].
+
+  Definition create_file_core (d : mfs_dir) (fn : string) :=
+    cwd <- Op LinkGetRoot;
+    f <?- create cwd (dir_to_pn d) fn;
+    Ret (Some f).
+
+
+  Ltac step_inv :=
+    match goal with
+    | H : LinkDirStableAPI.op_allow _ _ _ |- _ =>
+      inversion H; clear H; subst; repeat sigT_eq
+    | H : LinkAPI.step _ _ _ _ _ |- _ =>
+      inversion H; clear H; subst; repeat sigT_eq
+    | H : restricted_step _ _ _ _ _ _ _ |- _ =>
+      inversion H; clear H; subst; repeat sigT_eq
+    end.
+
+  Hint Extern 1 (LinkAPI.step _ _ _ _ _) => econstructor.
+  Hint Constructors LinkDirStableAPI.op_allow.
+
+
+  Theorem restricted_step_preserves_root :
+    forall tid `(op : LinkAPI.opT T) s r s',
+      restricted_step LinkAPI.step LinkDirStableAPI.op_allow op tid s r s' ->
+      FSRoot s = FSRoot s'.
+  Proof.
+    intros.
+    destruct H; intuition idtac; subst; eauto.
+    repeat step_inv; eauto.
+  Qed.
+
+  Theorem exec_others_preserves_root :
+    forall tid s s',
+      exec_others LinkAPI.step LinkDirStableAPI.op_allow tid s s' ->
+      FSRoot s = FSRoot s'.
+  Proof.
+    induction 1; intros; eauto.
+    repeat deex.
+    clear H0.
+    rewrite <- IHclos_refl_trans_1n; clear IHclos_refl_trans_1n.
+    clear H.
+    eapply restricted_step_preserves_root; eauto.
+  Qed.
+
+
+  Ltac exec_propagate :=
+    match goal with
+  (*
+    | s : RawLockAPI.State |- _ =>
+      destruct s
+  *)
+    | H : exec_any _ _ _ _ (Op _) _ _ |- _ =>
+      eapply exec_any_op in H; repeat deex
+    | H : exec_others _ _ _ ?s _,
+      Hi : context[FSRoot ?s] |- _ =>
+      rewrite (exec_others_preserves_root H) in Hi
+    end.
+
+  Ltac clear_allowed :=
+    match goal with
+    | H: LinkDirStableAPI.op_allow _ _ _ |- _ =>
+      clear H
+    end.
+
+
+  Theorem create_file_follows_protocol : forall tid s d fn,
+    follows_protocol_proc LinkAPI.step LinkDirStableAPI.op_allow LinkDirStableAPI.loopInv
+      tid s (create_file_core d fn).
+  Proof.
+    intros.
+    constructor; intros.
+      constructor. constructor.
+
+    repeat exec_propagate.
+    step_inv. clear_allowed. step_inv.
+
+    constructor; intros.
+    constructor; intros.
+    constructor; intros.
+    constructor; intros.
+    constructor. constructor.
+    destruct r; constructor.
+    destruct r; try constructor.
+    destruct n; try constructor.
+    destruct r; try constructor.
+    constructor.
+    destruct r; try constructor.
+  Qed.
+
+End Dirs.
+
 
 (* End-to-end layering plan:
 
@@ -34,12 +312,6 @@ Open Scope list.
 *)
 
 
-Definition maildir := "mail".
-Definition tmpdir := "tmp".
-
-Global Opaque maildir.
-Global Opaque tmpdir.
-
 Parameter tid_to_string : nat -> string.
 
 Definition starts_with_tid tid (name : string) : Prop :=
@@ -51,27 +323,24 @@ Inductive mailfs_step_allowed : forall T, linkOpT T -> nat -> LinkAPI.State -> P
 | MailAllowLinkAllocFile : forall dirnum name tid fs_state,
   starts_with_tid tid name ->
   path_eval_root fs_state [tmpdir] (DirNode dirnum) ->
+  (~ exists target, valid_link fs_state dirnum name target) ->
   mailfs_step_allowed (LinkAllocFile dirnum name) tid fs_state
 
 | MailAllowLinkLookupRoot : forall dirnum name tid fs_state,
   dirnum = FSRoot fs_state ->
-  proper_name name ->
   mailfs_step_allowed (LinkLookup dirnum name) tid fs_state
 
 | MailAllowLinkLookupTmp : forall dirnum name tid fs_state,
   starts_with_tid tid name ->
   path_eval_root fs_state [tmpdir] (DirNode dirnum) ->
-  proper_name name ->
   mailfs_step_allowed (LinkLookup dirnum name) tid fs_state
 
 | MailAllowLinkLookupMail : forall dirnum name tid fs_state,
   path_eval_root fs_state [maildir] (DirNode dirnum) ->
-  proper_name name ->
   mailfs_step_allowed (LinkLookup dirnum name) tid fs_state
 
 | MailAllowLinkLookupUser : forall dirnum name tid fs_state user f,
   path_eval_root fs_state [maildir; user] (DirNode dirnum) ->
-  proper_name name ->
   valid_link fs_state dirnum name (FileNode f) ->
   mailfs_step_allowed (LinkLookup dirnum name) tid fs_state
 
@@ -123,22 +392,19 @@ Definition unique_dir_pn (fs : FS) :=
     path_eval_root fs pn1 (DirNode d) ->
     pn0 = pn1.
 
-Definition unique_pn_dir (fs : FS) :=
-  forall pn d1 d2,
-    path_eval_root fs pn (DirNode d1) ->
-    path_eval_root fs pn (DirNode d2) ->
-    d1 = d2.
+Definition unique_pn_node (fs : FS) :=
+  forall pn n1 n2,
+    path_eval_root fs pn n1 ->
+    path_eval_root fs pn n2 ->
+    n1 = n2.
+
+Definition exists_dir (fs : FS) (pn : Pathname) :=
+  exists dirnum,
+    path_eval_root fs pn (DirNode dirnum).
 
 Definition invariant (fs : FS) :=
   unique_dir_pn fs /\
-  unique_pn_dir fs /\
-  unique_pathname_root fs [tmpdir] /\
-  proper_pathname_root fs [tmpdir] /\
-  unique_pathname_root fs [maildir] /\
-  proper_pathname_root fs [maildir] /\
-  forall user,
-    maybe_unique_pathname_root fs [maildir; user] /\
-    proper_pathname_root fs [maildir; user].
+  unique_pn_node fs.
 
 
 Module MailLinkAPI <: Layer.
